![[WhatsApp Image 2023-02-18 at 3.58.46 PM.jpeg]]
CORECTION 
![[Pasted image 20230219140605.png]]
1) X/180 = Y/$\pi$ 
y/$\pi$ = 33/180
y= 11/60$\pi$ 
2) $3\pi/8$ = 
x/180 = y/$\pi$  
x/180 = 3$\pi/8/\pi$ 
x = 3/8 x 180
x= 67.5 
3) y/$\pi$ = 135/180
y = 3/4$\pi$ 
![[Pasted image 20230219141344.png]]
7$\pi$ = $\pi$ 
110$\pi$ /3 = 111$\pi$ - $\pi$ / 3 = $\pi$/3
19$\pi$ / 4 = 20$\pi$ - $\pi$ /4 = $\pi$ / 4 
131 $\pi$ / 3 = 132$\pi$ - $\pi$ / 3 = $\pi$ / 3
217$\pi$ / 6 = 36$\pi$ - 217$\pi$ /6 = -$\pi$ / 6 
![[Pasted image 20230219144104.png]]
$cos10\pi/3$ = cos ($\pi$+7$\pi$/3) = 7$\pi$/3 = $6\pi$ + $\pi$ / 3 
cos ($\pi+\pi/3$ ) = -cos($\pi/3$ ) = -1/2

sin 53$\pi$ /6 = 48$\pi$ +5$\pi$ /6 = 5$\pi$ /6
sin(5$\pi$/6) = sin ($\pi$/2+$\pi$/3) = -sin($\pi/3$) = -$\sqrt{3/2}$  

cos 34$\pi$ / 3 = 30$\pi+4\pi$ / 3 = cos ($\pi$ +$\pi/3$ ) 
 cos ($\pi$ +$\pi/3$ ) = cos ($\pi$/3) = -1/2

cos 13$\pi$ / 6 = 12$\pi$ + $\pi$ / 6 = cos ($\pi$/6) = $\sqrt{3/2}$  

tan 37$\pi$ / 4 = 32$\pi+5\pi/4$ = tan ($\pi+\pi/4$ ) =
tan($\pi$/4) = 1

![[Pasted image 20230219150927.png]]

on sait que $1+tan(x) = 1/cos(x)$ 
donc 1 + ($tanx^{2}$ = $1/cosx^{2}$ )

ex 8
tan x = 1/3 et $\pi/2$ < x < $\pi$ 

on sait que tan x = sin x/ cos x 
donc cos x = sin x / tan x
cos x = $1-cos^{2}x / 1/3$ 
cos x = $3 sin^{2}x$ = 3cosx

sin x = tan$x$ x cos$x$ 
sin x = 1/3 x $3 cosx$ 
sin x = - sin (x) = -cos x 
![[Pasted image 20230224155953.png]]
1) on a $cos^{2}x$ = 1-$sin^{2}x$ 
$cos^{2}x$ = 1-(-4/5)
$cos^{2}x$ =9/5
on sait que tanx=sinx/cosx
tan x = -4/5 / 9/5 = -4/9 
2) on a 
$cos^{2}x$ = 1-$sin^{2}x$ 
= 1-$\sqrt{2/3}$ 
cos x = 3-$\sqrt{6}$ / 3
tan x = sin x / cox x 
tan x = $\sqrt{6}$ + 2
3) ona tan x = sin x / cos x
et 1+tan x = 1/cos x
1/cos x = 1+$2\sqrt{3}$ 
cos x = -1-$2\sqrt{3}$ 
et sin x = $tanx.cosx$  
sin x = $\sqrt{2/3}$ . 1-$2\sqrt{3}$ 
sin x = $\sqrt{6}$ -6$\sqrt{3}$ /3

![[Pasted image 20230224162858.png]]
A = sin ($\pi-x$ ) x cos ( $\pi/2 - x$) - sin ($\pi/2 - x$) x cos($\pi-x$ ) 
a = sin(x) . sin (x) - cos x (-cos(x))
a = $sin^{2}x + cos^{2}x$ 
a = 1 
B = sinx+sinx / -cos x
b = 2sinx / -cos x 
C= 
cos ($\pi/2 + \pi/3$ ) + sin($\pi/2 + \pi/3$ ) - tan($\pi/2 + \pi/3$ )
c= -sin x + cos x - (-1/tanx)
D= 
sin ($\pi - x$ ) + cos ($\pi+x$ ) + cos($\pi-x$ )
d = sin x - cos x - cos x 
d = sin x - 2cos x
e= 
tan ($\pi-x$  ) + tan ($\pi+x$ )
e = -tan x +tan x 
e = 0
H= $sin^{2}$ ($\pi/8$ ) + $sin^{2}$ ($3\pi/8$ ) +$sin^{2}$ {$\pi/2 + \pi/8$ } + $sin^{2}$ + ($\pi/2 + 3\pi/8$ )
H=$sin^{2}$ ($\pi/8$ ) + $sin^{2}$ ($3\pi/8$ )  + $cos^{2}$ ($\pi/8$) + $cos^{2}$ ($3\pi/8$)
h = 1 + 1 
h = 2 
